experiment/Experiment.Steel.Test.Extract.fst
@@ -22,6 +22,13 @@ let test3_LV (r0 r1 : ref U32.t)
       (ensures fun h0 () h1 -> U32.v (sel r1 h1) == U32.v (sel r0 h0) + 1)
   = Test.test3_LV r0 r1 ()
 
+let test3_LV' (r0 r1 : ref U32.t)
+  : Steel unit
+      (vptr r0 `star` vptr r1) (fun _ -> vptr r0 `star` vptr r1)
+      (requires fun h0 -> U32.v (sel r0 h0) < 42)
+      (ensures fun h0 () h1 -> U32.v (sel r1 h1) == U32.v (sel r0 h0) + 1)
+  = Test.test3_LV' r0 r1 ()
+
 
 let test_ghost (r : ref U32.t)
   : Steel U32.t (vptr r) (fun _ -> vptr r)
